SepLogicTime/Splay_Tree_Impl.thy
@@ -97,26 +97,30 @@ partial_function (heap) splay_impl :: "'a::{heap,linorder} \<Rightarrow> 'a ptre
 declare splay_impl.simps [sep_proc]
 
 setup {* fold add_rewrite_rule @{thms splay.simps} *}
-setup {* add_fun_induct_rule (@{term t_splay}, @{thm t_splay.induct}) *}
 
-definition splay_time :: "'a::linorder \<Rightarrow> 'a tree \<Rightarrow> nat" where
+definition splay_time :: "'a::linorder \<Rightarrow> 'a tree \<Rightarrow> nat" where [rewrite]:
   "splay_time a t = 15 * t_splay a t"
 
-lemma splay_time_simps [rewrite]:
+lemma splay_time_simp:
   "splay_time a Leaf = 15"
-  "splay_time a \<langle>l, a, r\<rangle> = 15"
-  "a<b \<Longrightarrow> splay_time a \<langle>Leaf, b, r\<rangle> = 15"
-  "a<b \<Longrightarrow> splay_time a \<langle>\<langle>ll, a, lr\<rangle>, b, r\<rangle> = 15"
-  "a<b \<Longrightarrow> a<c \<Longrightarrow> splay_time a \<langle>\<langle>ll, c, lr\<rangle>, b, r\<rangle> =
-   (if ll = Leaf then 15 else splay_time a ll + 15)"
-  "a<b \<Longrightarrow> c<a \<Longrightarrow> splay_time a \<langle>\<langle>ll, c, lr\<rangle>, b, r\<rangle> =
-   (if lr = Leaf then 15 else splay_time a lr + 15)"
-  "b<a \<Longrightarrow> splay_time a \<langle>l, b, Leaf\<rangle> = 15"
-  "b<a \<Longrightarrow> splay_time a \<langle>l, b, \<langle>rl, a, rr\<rangle>\<rangle> = 15"
-  "b<a \<Longrightarrow> a<c \<Longrightarrow> splay_time a \<langle>l, b, \<langle>rl, c, rr\<rangle>\<rangle> =
-  (if rl=Leaf then 15 else splay_time a rl + 15)"
-  "b<a \<Longrightarrow> c<a \<Longrightarrow> splay_time a \<langle>l, b, \<langle>rl, c, rr\<rangle>\<rangle> =
-  (if rr=Leaf then 15 else splay_time a rr + 15)" by (simp add: splay_time_def)+
+  "splay_time a (tree.Node l b r) =
+    (if a = b then 15
+     else if a < b
+          then case l of
+            Leaf \<Rightarrow> 15 |
+            tree.Node ll c lr \<Rightarrow>
+              (if a=c then 15
+               else if a < c then if ll = Leaf then 15 else splay_time a ll + 15
+                    else if lr = Leaf then 15 else splay_time a lr + 15)
+          else case r of
+            Leaf \<Rightarrow> 15 |
+            tree.Node rl c rr \<Rightarrow>
+              (if a=c then 15
+               else if a < c then if rl = Leaf then 15 else splay_time a rl + 15
+                    else if rr = Leaf then 15 else splay_time a rr + 15))"
+  by (auto split!: tree.split simp: splay_time_def)
+setup {* fold add_unfolding_rule @{thms splay_time_simp} *}
+setup {* add_fun_induct_rule (@{term t_splay}, @{thm t_splay.induct}) *}
 
 lemma splay_not_Leaf: "splay x \<langle>l, a, r\<rangle> \<noteq> Leaf" by auto
 setup {* add_forward_prfstep_cond @{thm splay_not_Leaf} [with_term "splay ?x \<langle>?l, ?a, ?r\<rangle>"] *}
@@ -126,7 +130,9 @@ lemma splay_correct [hoare_triple]:
     splay_impl x a
    <btree (splay x t)>\<^sub>t"
 @proof @fun_induct "t_splay x t" arbitrary a @with
+  @subgoal "(x = x, t = Leaf)" @unfold "splay_time x Leaf" @endgoal
   @subgoal "(x = x, t = \<langle>lt, b, rt\<rangle>)"
+  @unfold "splay_time x \<langle>lt, b, rt\<rangle>"
     @case "x = b"
     @case "x < b" @with
       @case "lt = Leaf"
